proved a few lemmas for contact graphs: add_nodeN, add_nodeS, and remove_nodeN

ContactGraph.v
@@ -39,6 +39,12 @@ Notation "p1 =sym= p2" := (eq_sym p1 p2)
   (at level 70, no associativity).
 
 (* finite maps *)
+(* Extra lemmas for finite maps.
+ * One of them will be soon integrated into mathcomp.finmap: codomf_cat.
+ * codomf_const: codomf of constant map.
+ * setksD: setks and domf.
+ * setksC: setks and codomf.
+ *)
 Section FinMap.
 Variables (K V : choiceType).
 
@@ -102,6 +108,7 @@ Section CG.
 Variable (g : cg).
 Definition nodes : {fset N} := codomf (siteMap g).
 Definition sites : {fset S} := domf (siteMap g).
+Definition sites_of (n : N) : {fset S} := getks (siteMap g) n.
 
 Definition add_site (s : S) (to_n : N) : cg :=
   @CG (siteMap g).[s <- to_n] (edges g) (edges_sym g).
@@ -126,7 +133,7 @@ Definition remove_sites (ss : {fset S}) : cg :=
   @CG (siteMap g).[\ ss] (edges g) (edges_sym g).
 
 Definition remove_node (n : N) : cg :=
-  remove_sites (getks (siteMap g) n).
+  remove_sites (sites_of n).
 
 Definition remove_edge (s t : S) : cg.
   pose es x y := if (x, y) =sym= (s, t) then false else @edges g x y.
@@ -141,21 +148,110 @@ End CG.
 End NS.
 
 
+(* Lemmas for contact graphs.
+ * add_nodeN: add_node and nodes.
+ * add_nodeS: add_node and sites.
+ * remove_nodeN: add_node and nodes.
+ * remove_nodeS: add_node and sites.
+ *)
 Module Lemmata.
 Section CG_NS.
 Variables (N S : choiceType) (g : cg N S).
 
-Lemma nodesN (n : N) (ss : {fset S}) :
+Lemma add_nodeN (n : N) (ss : {fset S}) :
   ss != fset0 ->
   nodes (add_node g n ss) = n |` nodes (remove_sites g ss).
-Proof using Type.
-  rewrite /nodes /add_node /=. apply: setksC.
-Qed.
+Proof using Type. apply: setksC. Qed.
 
-Lemma smN (n : N) (ss : {fset S}) :
-  siteMap (add_node g n ss) = siteMap g.
+Lemma add_nodeS (n : N) (ss : {fset S}) :
+  sites (add_node g n ss) = sites g `|` ss.
+Proof using Type. by rewrite /sites /= fsetUDr fsetDv fsetD0. Qed.
+
+Lemma notin_sites (n1 n2 : N) (s : sites g) :
+  (siteMap g s == n1) && (n1 != n2) ->
+  fsval s \notin sites_of g n2.
 Proof using Type.
 Admitted.
+
+Lemma notin_sites' (n : N) (s : sites g) :
+  fsval s \notin sites_of g n -> siteMap g s != n.
+Proof using Type.
+Admitted.
+
+Lemma remove_nodeN (n : N) :
+  nodes (remove_node g n) = nodes g `\ n.
+Proof using Type.
+  rewrite /remove_node /nodes.
+  (* rewrite codomf_rem_exists. *)
+  rewrite codomf_rem. Locate "\notin".
+  Search "fset" "eq_". About Imfset.imfset.
+  apply/fsetP => x. apply/imfsetP.
+  case: ifP => /=. Locate "exists2".
+  (* use x to get the a site of x: *)
+  (* if x is in codomf (siteMap g) then there must be a site *)
+  (* mapping to it in domf (siteMap g). *)
+  Search (_ \in _ `\ _).
+  Search (_ \in codomf _). Search "fset" (_ \in _).
+  (* rewrite in_fsetD1 => /andP[xNEn xIc]. *)
+  (* rewrite in_fsetD1 => /andP[xNEn /codomfP[s Hs]]. *)
+  rewrite in_fsetD1 mem_codomf => /andP[xNEn /existsP[s Hs]].
+  exists s. Locate "pred". About SimplPred. rewrite inE.
+  apply (@notin_sites x n s).
+  - by rewrite xNEn Hs.
+  - by rewrite (eqP Hs).
+  move=> /negbT xNIcod [s sNSOn] sSOx.
+  (* the proof proceeds by showing that x == n *)
+  rewrite inE in sNSOn.
+  Search (_ ?x = _) codomf. About mem_codomf.
+  have xIcod: x \in codomf (siteMap g).
+  { rewrite mem_codomf. apply/existsP.
+    exists s. by rewrite sSOx. }
+  rewrite !inE in xNIcod.
+  apply/negP: xNIcod. rewrite negbK. apply/andP. split; last first.
+  apply/existsP. exists s. by rewrite sSOx.
+  (* by sNSOn, siteMap g s != n *)
+  (* have H (n1 : N) (s1 : sites g) : *)
+  (*   reflect (fsval s1 \in sites_of g n1) (siteMap g s1 == n1). *)
+  (* have H (n1 : N) (s1 : sites g) : *)
+  (*   fsval s1 \in sites_of g n1 <-> siteMap g s1 == n1. *)
+  rewrite sSOx.
+  apply: notin_sites'. by apply: sNSOn.
+Qed.
+  (* suff sID: forall s : S, *)
+  (*     s \in sites_of g n -> s \in domf (siteMap g). *)
+  (* suff H: forall s : S, forall h : s \in sites_of g n, *)
+  (*     siteMap g [` sID s h] = n. *)
+  (* suff H1: forall v : N, *)
+  (*     [exists k, (val k \notin sites_of g n) && *)
+  (*                  (siteMap g k == v)] = *)
+  (*       (v != n). *)
+
+Lemma imfset_id' (X : {fset N}) : [fset x | x in X] = X.
+Proof using Type. by rewrite imfset_id. Qed.
+
+Search "fset" reflect.
+
+Lemma b (X : {fset N}) (n : N) :
+  [fset x | x in X & x != n] = X `\ n.
+Proof using Type.
+  apply/fsetP => x'. symmetry. About fsetD1P. apply/fsetD1P.
+Admitted.
+
+Lemma sites_ofDM (s : S) (n : N) :
+  s \in sites_of g n -> s \in domf (siteMap g).
+Proof using Type.
+Admitted.
+
+Lemma sites_ofM (s : S) (n : N) (H : s \in sites_of g n) :
+  siteMap g [` sites_ofDM H] = n.
+Proof using Type.
+Admitted.
+
+Lemma remove_nodeS (n : N) :
+  sites (remove_node g n) = sites g `\` sites_of g n.
+Proof using Type.
+Admitted.
+
 
 End CG_NS.
 End Lemmata.
